invariants seem to check out

proof/spec/extra/SpecSecurity.ec
@@ -62,43 +62,110 @@ op pkrel(apk : pkXMSSTW, pk : xmss_pk) =
    (* apk.`3 = ??? Why is the address in the sk/pk? *)
    (* ??? = pk.`pk_oid I guess abstract proofs fon't care about oid *).
 
+(* Notes:
+- We have a full binary tree with height h+1, so 2^h nodes.
+- Levels are indexed from bottom to top, leaves at level 0, root at level h
+- The length of a full path to a leaf is h
+- The length of the path to a node at level l \in [0..h] is h - l (root path is [])
+- The path to a leaf can be extracted from the bit representation of its index:
+    the i-th leaf can be found at path rev (bits h i)
+- throughout we will need the corner case of the leaf with index 2^h when
+  we exit the loop, where everything works in a tree of height h+2
+*)
+
 (* The hamming weight of a path determines the size of the stack *)
-op hw(p : bool list) = size (filter idfun p).
+op hw(p : bool list) = count (pred1 true) p.
 
 (* The path of a leaf; we need the corner case of leaf 2^h for exiting the loop *)
 op lpath(lidx : int) = rev (BS2Int.int2bs (if lidx = 2^h then (h+1) else h) lidx).
 
-(* The paths of all the nodes corresponding to one bits in a leaf path *)
+(* The paths of all the sibling nodes of 1-bit choices in a leaf path *)
 op paths_from_leaf(lidx : int) : bool list list = 
-   foldl (fun (paths : bool list list) (bi : _*_) => 
+   if (lidx = 2^h) then [[]] (* we get the root *)
+   else pmap (fun (bi : _*_) => 
      if bi.`1 
-     then paths ++ [(take bi.`2 (lpath lidx)) ++ [false]] 
-     else paths) [] (zip (lpath lidx) (iota_ 0 h)).
+     then Some ((take bi.`2 (lpath lidx)) ++ [false])
+     else None) (zip (lpath lidx) (iota_ 0 h)).
+
+lemma size_lpath (lidx) :
+   lidx <= 2^h =>
+     size (lpath lidx) = if lidx = 2^h then (h+1) else h.
+move => H. 
+rewrite /lpathl size_rev BS2Int.size_int2bs; smt(h_g0).   
+qed.
+
+lemma pfl_size (lidx : int) :
+   lidx <= 2^h =>
+   size (paths_from_leaf lidx) = hw (lpath lidx).
+rewrite /paths_from_leaf => Hs.
+case (lidx = 2 ^ h) => /= Hh.
++ rewrite /lpath /= Hh /= /hw BS2Int.int2bs_pow2;1:smt(mem_range h_g0).
+  have -> : (h + 1 - 1 - h) = 0 by ring.
+  rewrite nseq0 /= rev_cat rev1 count_cat /pred1 /= /b2i /=.
+  rewrite (eq_in_count _ pred0);1: by move => x;rewrite rev_nseq mem_nseq /#.
+  by rewrite count_pred0 /=.
+rewrite /hw.
+have -> : h = size (lpath lidx) by smt(size_lpath).
+rewrite pmap_map size_map size_filter.
+admit.
+qed.
 
 (* The list of leaves that are under a node given by a path *)
 op leaves_from_path(p : bool list) =
-   let hsub = h - size p in
-   let start = foldl (fun i acc => acc + 2^i) 0 (iota_ 0 (hw p)) in 
-   iota_ start (2^hsub).
+   if size p = h+1 then witness (* we should never need this *)
+   else
+     let hsub = h - size p in
+     let start = foldl (fun acc (bi : _ * _) => acc + if bi.`1 then 2^(h - bi.`2) else 0) 0 (zip p (iota_ 0 (size p))) in 
+         iota_ start (2^hsub).
 
-(* The leaf node corresponding to a leaf path *)
+lemma lfp_leaf lidx :
+  lidx < 2^h =>
+  (leaves_from_path (lpath lidx)) = [lidx].
+move => Hh.
+rewrite /leaves_from_path ifF /=. admit.
+rewrite size_lpath 1:/# /= ifF 1:/# /= iota1;congr.
+admit. 
+qed.
+
+(* The leaf node corresponding to a leaf path
+   The semantics of this needs to be computed from wots using
+   operators and then proved equivalent to the imperative code. *)
 op leafnode_from_idx(ss ps : Params.nbytes, ad : SA.adrs, lidx : int) : dgstblock.
 
-(* all the leaves up to an index *)
+(* list of all the leaves up to an index, exclusive *)
 op leaf_range(ss ps : Params.nbytes, ad : SA.adrs, lidx : int) =
-   map (leafnode_from_idx ss ps ad) (iota_ 0 (lidx+1)).
+   map (leafnode_from_idx ss ps ad) (iota_ 0 lidx).
 
-(* The node corresponding to a path *)
+(* The node corresponding to an arbitrary path  *)
 op node_from_path(p : bool list,ss ps : Params.nbytes, ad : SA.adrs) : dgstblock =
-   let ls = leaves_from_path p in
-     let nls = map (leafnode_from_idx ss ps ad) ls in
-     let subtree = list2tree nls in
-        (val_bt_trh subtree ps (set_typeidx ad trhtype) (h - size p) (head witness ls)).
+   if size p = h+1 then witness (* we should never need this *)
+   else 
+      let ls = leaves_from_path p in
+      let nls = map (leafnode_from_idx ss ps ad) ls in
+      let subtree = list2tree nls in
+         (val_bt_trh subtree ps (set_typeidx ad trhtype) (h - size p) (head witness ls)).
 
 (* The full stack state when one starts to process leaf lidx *)
 op stack_from_leaf(lidx : int,ss ps : Params.nbytes, ad : SA.adrs) : (dgstblock * int) list = 
    map (fun p =>
      (node_from_path p ss ps ad, (h - size p))) (paths_from_leaf lidx).
+
+
+lemma sfl_size lidx ss ps ad :
+  lidx <= 2^h =>
+  size (stack_from_leaf lidx ss ps ad) = hw (lpath lidx).
+proof.
+move => Hi.
+rewrite  /stack_from_leaf size_map /paths_from_leaf.
+case (lidx = 2 ^ h) => H /=.
++ rewrite /lpath /= H /= /hw BS2Int.int2bs_pow2;1:smt(mem_range h_g0).
+  have -> : (h + 1 - 1 - h) = 0 by ring.
+  rewrite nseq0 /= rev_cat rev1 count_cat /pred1 /= /b2i /=.
+  rewrite (eq_in_count _ pred0);1: by move => x;rewrite rev_nseq mem_nseq /#.
+  by rewrite count_pred0 /=.
+rewrite pmap_map size_map size_filter /hw /predC1 /= count_map /preim /=.
+admit.
+qed.
 
 (* The list of leaves that fall under the first node in the stack when one starts to process leaf lidx
    The case o lidx=0 is a corner case, as the stack is empty *)
@@ -111,30 +178,35 @@ op first_subtree_leaves(lidx : int,ss ps : Params.nbytes, ad : SA.adrs) =
 
 (* The hamming weight of 0 is 0, so stack is empty *)
 lemma pfl0 : paths_from_leaf 0 = [].
-rewrite /paths_from_leaf.
-rewrite (foldl_in_eq (fun (paths : bool list list) (bi : bool * int) =>
-     if bi.`1 then paths ++ [take bi.`2 (lpath 0) ++ [false]] else paths) (fun (paths : bool list list) (bi : bool * int) => paths)).
-+ move => path;rewrite /lpath =>  bi H /=.
-  have := mem_zip  (lpath 0) (iota_ 0 h) bi.`1 bi.`2 _;1:smt().
-  rewrite /lpath mem_rev BS2Int.int2bs0 mem_nseq /#.
-  by elim (zip (lpath 0) (iota_ 0 h)) => //=.
+rewrite /paths_from_leaf ifF;1:smt(StdOrder.IntOrder.expr_gt0 h_g0). 
+rewrite (eq_in_pmap _ (fun _ => None)).
++ move => bi H; have := mem_zip  (lpath 0) (iota_ 0 h) bi.`1 bi.`2 _; 1:smt().
+  rewrite /lpath mem_rev BS2Int.int2bs0 mem_nseq /#. 
+by apply pmap_none.
 qed.
 
 (* This op describes the state of the stack in the inner loop, while
    reducing, where i is the number of the iteration we are in.
+   At iteration zero we just added the leaf we are processing (lidx) to 
+   the stack.
    The loop performs as many iterations as needed to reduce the 
-   hamming weight of lidx to hamming weight of lidx+1, which may
-   be no iterations at all if the hamming weight increases *)
-search belast.
+   hamming weight of lidx to hamming weight of lidx+1, if any. *)
 op stack_increment(lidx : int,ss ps : Params.nbytes, ad : SA.adrs, i : int) =
   let hwi = hw (lpath lidx) in
   let hwi1 = hw (lpath (lidx + 1)) in
-  if hwi < hwi1 then stack_from_leaf (lidx+1) ss ps ad
+  if hwi < hwi1 
+  (* Then then case only happens when lidx is even, in which
+     case we are already in the state we need on exit *)
+  then stack_from_leaf (lidx+1) ss ps ad
   else 
-      let red = hwi - hwi1 in
-      let lps = (paths_from_leaf lidx) in
-      let lps1 = (paths_from_leaf (lidx+1)) in
-      (* we still did not touch positions [0 ... (hwi1 - 1 + red - i)] *)
+      (* reducing red positions requires red+1 hashes
+         i must be in the range 0<=i<=red if loop is entered.
+         when i = 0 the stack has size hwi + 1
+         when i = red+1,i.e., we exit the loop, the stack has size hwi1 
+         at any i when we enter the loop we have still
+         not touched positions 0..hwi1+red-1-i in the stack *)
+      let red = hwi - hwi1 in 
+      (* we still did not touch positions [0 ... (hwi1 + red - 1 - i)] *)
       (* and the stack contains only one more element in position      *)
       (* (hwi1 + red - i) that corresponds to the node along the path to
          lidx that we can also compute *)
@@ -161,8 +233,8 @@ sp 7 14;wp;conseq
     (: _ ==> (val_bt_trh (list2tree leafl0{1}) ps{1} (set_typeidx (XAddress.val witness) trhtype) h 0 =
               DigestBlock.insubd (BytesToBits (NBytes.val (nth witness stack{2} 0))))).
 + by auto => /> &1 *;smt(NBytes.valK). print dgstblock.
-while (size leafl0{1} = i{2} /\ 0 <= i{2} <= 2^h 
-    /\ leafl0{1} = leaf_range  ss{1} ps{1} ad{1} (i{2}-1) 
+while (size leafl0{1} = i{2} /\ 0 <= i{2} <= 2^h /\ t{2} = h 
+    /\ leafl0{1} = leaf_range  ss{1} ps{1} ad{1} i{2} 
     /\ (let firstleaves = first_subtree_leaves i{2} ss{1} ps{1} ad{1} in
            take (size firstleaves) leafl0{1} = firstleaves)
     /\ (let stacklist = stack_from_leaf i{2} ss{1} ps{1} ad{1} in 
@@ -177,22 +249,124 @@ while (size leafl0{1} = i{2} /\ 0 <= i{2} <= 2^h
   + by rewrite /leaf_range iota0 /=.  
   + by rewrite /stack_from_leaf pfl0 /= /#.
   + by move => h ?; rewrite /stack_from_leaf pfl0 /= /#.
-  + move => leafs1 hs1 o1 st2 ???????H.
-   have Hlp : (lpath (size leafs1)) = true :: nseq h false.
-   + rewrite /lpath.
-     have -> /= : (size leafs1) = 2^h by smt().
-     rewrite BS2Int.int2bs_pow2 /=;1:smt(mem_range h_g0).
-     by rewrite nseq0 /= rev_cat rev_nseq rev1 cat_cons /=.
-    move : (H 0 _) => /=. 
-    + rewrite /= /stack_from_leaf size_map /paths_from_leaf /=. 
-      rewrite Hlp.
-      rewrite iotaS_minus /=;1:smt(h_g0). admit.
-  rewrite /bs2block => ->.
-  rewrite /stack_from_leaf nth0_head /paths_from_leaf /=.
-  rewrite Hlp /=.
-  admit. 
+  + move => leafs1 hs1 o1 st2 ????Hl??H.
+    move : (H 0 _) => /=;1: by smt().
+    rewrite /bs2block => ->.
+    rewrite /stack_from_leaf nth0_head /paths_from_leaf /=.
+    rewrite ifT 1:/# /=. 
+    rewrite /node_from_path /= /leaves_from_path !ifF /=;1,2:smt(h_g0).
+    congr;last first.
+    + rewrite iotaS_minus /=;1:smt(StdOrder.IntOrder.expr_gt0).
+      by rewrite /hw /= /idfun /= iota0 //.
+    + congr;rewrite Hl.
+      rewrite /leaf_range;congr.
+      rewrite /hw /= /idfun /= (iota0 0 0) //= /#. 
 
-admitted.
+seq 3 6 : (#pre /\ 
+  leaf{1} = leafnode_from_idx ss{1} ps{1} ad{1} i{2} /\ leaf{1} = bs2block node{2}). 
+  admit. (* this can be fixed by setting leafnode_from_idx to the correct semantics *)
+
+wp.
+while {2} ((hw (lpath i{2}) < hw (lpath (i{2} + 1)) => to_uint offset{2} = hw (lpath (i{2} + 1))) /\
+           (hw (lpath (i{2} + 1)) <= hw (lpath i{2}) => hw (lpath (i{2} + 1)) <= to_uint offset{2} <= hw (lpath i{2})) /\
+    i{2} = size leafl0{1} /\
+    0 <= i{2} < 2 ^ h /\
+    t{2} = h /\
+    leafl0{1} = leaf_range ss{1} ps{1} ad{1} i{2} /\
+    (let firstleaves = first_subtree_leaves i{2} ss{1} ps{1} ad{1} in 
+         take (size firstleaves) leafl0{1} = firstleaves) /\
+    let stacklist = stack_increment i{2} ss{1} ps{1} ad{1} (to_uint offset{2} - (hw (lpath i{2})) - 1) in
+        to_uint offset{2} = size stacklist /\
+      forall (k : int),
+        0 <= k < size stacklist =>
+          bs2block (nth witness stack{2} k) = (nth witness stacklist k).`1 /\
+          to_uint (nth witness heights{2} k) = (nth witness stacklist k).`2 /\
+  leaf{1} = leafnode_from_idx ss{1} ps{1} ad{1} i{2} /\ leaf{1} = bs2block node{2})
+    (to_uint offset{2}); last first. 
++ auto => /> &1 &2 ????Ho Hs??Hn; pose _lidx := size leafl0{1};do split.
++ admit. (* hw property *)
++ admit. (* hw property *)
++ rewrite !to_uintD_small /=. admit. (* we need an upper bound on h *)
+  rewrite Ho /stack_increment /=.
+  case (hw (lpath _lidx) < hw (lpath (_lidx + 1))).
+  + admit. (* hw increases by exactly 1*)
+  move => ?;rewrite -/_lidx.
+  pose _olds := (stack_from_leaf _lidx ss{1} ps{1} ad{1}).
+  pose _hw1 := (hw (lpath (_lidx + 1))).
+  pose _hw := (hw (lpath (_lidx))).
+  have Hsos : size _olds = _hw
+   by rewrite /olds /stack_from_leaf size_map; smt(pfl_size h_g0). 
+  rewrite Hsos /=.
+  have -> : (_hw1 + (_hw - _hw1) - (_hw + 1 - _hw - 1)) = _hw by ring.
+  have -> /= : (h - (_hw + 1 - _hw - 1)) = h by ring.
+  rewrite size_cat /= size_take /=;1:by smt(count_ge0). 
+  by smt().
++ move => k kbl.
+  have -> : (offset{2} + W64.one - W64.one) = offset{2} by ring.
+  rewrite /= !to_uintD_small;1: admit. (* we need an upper bound on h *)
+  move => kbh; move :  (Hs k _). admit. (* lemma that stack decreases in reduction *)
+  move => [H1 H2].
+  have -> : (to_uint offset{2} + to_uint W64.one - hw (lpath _lidx) - 1)    = 0.
+  + rewrite Ho /=.
+    have -> : size (stack_from_leaf (size leafl0{1}) ss{1} ps{1} ad{1}) = hw (lpath _lidx);last by ring.
+    by smt(sfl_size h_g0).
+  rewrite /stack_increment /=.
+  pose _olds := (stack_from_leaf _lidx ss{1} ps{1} ad{1}).
+  pose _hw1 := (hw (lpath (_lidx + 1))).
+  pose _hw := (hw (lpath (_lidx))).
+  have Hsos : size _olds = _hw
+      by rewrite /olds /stack_from_leaf size_map; smt(pfl_size h_g0). 
+  have -> : take (_hw1 + (_hw - _hw1)) _olds = _olds.
+  + have -> : (_hw1 + (_hw - _hw1)) = size _olds by smt().
+    by rewrite take_size.
+  have -> : node_from_path (take h (lpath _lidx)) ss{1} ps{1} ad{1} = bs2block node{2}. 
+  + rewrite -Hn /node_from_path /= ifF ;1: smt(size_take h_g0).
+    have -> : (take h (lpath _lidx) = (lpath _lidx));1: smt(take_size BS2Int.size_int2bs h_g0 size_rev). 
+    rewrite lfp_leaf /=;1:smt().
+    rewrite -/_lidx size_lpath /=;1:smt().
+    rewrite ifF 1:/# /list2tree /= ifT;1: by exists 0 =>/=.
+    admit. (* we need to know that evaluation at level 0 is the leaf *)
+  + (* this is the initialization of the inner loop *)
+    case (_hw < _hw1) => /= *.
+    + (* hw increased by 1, so we have to show that the previous stack plus
+         the new leaf is really the stack that we will end up with *)
+      admit. 
+    + (* reductions will be needed, but we haven't started, 
+         so we have the old stack in the first positions and a 
+         new leaf at the next position *)
+      rewrite !nth_cat.
+      case (k < size _olds) => *;1: smt(sfl_size nth_put).
+      rewrite !ifT. admit. 
+      rewrite !size_take /=; 1:smt(h_g0).
+      rewrite !size_lpath /=;1:smt(). 
+      rewrite !ifF /=;1..3:smt(). 
+      have -> : k = to_uint offset{2}. 
+      + have ? : to_uint offset{2} = _hw by smt(sfl_size).
+        move : kbh.
+        have -> : (to_uint offset{2} + to_uint W64.one - hw (lpath _lidx) - 1) = to_uint offset{2} - _hw by rewrite /=;smt().
+        rewrite /stack_increment /= ifF 1:/#.
+        rewrite -/_hw -/_hw1 -/_lidx size_cat /=.
+        have -> : (_hw1 + (_hw - _hw1) - (to_uint offset{2} - _hw))= _hw by smt().
+        rewrite size_take;1: smt(count_ge0). 
+        smt(sfl_size).
+      rewrite !nth_put /=. admit. admit. 
+      done.
+     
+move => hs o2 s2;do split => H H0 H1 H2 H3. 
++ rewrite /(\ule) /= H1.  admit.  (* something about termination condition? *)
++ do split. 
+  + smt(size_rcons). 
+  + smt().
+  + smt().
+  + admit. (* to do *)
+  + admit. (* to do  *) 
+  + admit. (* to do *) 
+  + admit. (* to do *)
+  + admit. (* to do *)
+
+move => *. 
+admit. (* preservation of inner loop invariant *)
+qed.
 
 (* Signature type is abused with two index copies because I need this to simulate
    the actual operation of the implementation *)
